Parse domain

src/RawAst/RawAst.dfy
@@ -7,7 +7,13 @@ module RawAst {
   // Top-level program
 
   // A raw program reflects program that has been parsed.
-  datatype Program = Program(types: seq<TypeName>, taggers: seq<Tagger>, functions: seq<Function>, axioms: seq<Axiom>, procedures: seq<Procedure>)
+  datatype Program = Program(
+    domains: seq<Domain>,
+    types: seq<TypeName>,
+    taggers: seq<Tagger>,
+    functions: seq<Function>,
+    axioms: seq<Axiom>,
+    procedures: seq<Procedure>)
   {
     // A raw program is well-formed when its identifiers resolve to declarations and some basic
     // properties hold:
@@ -40,6 +46,15 @@ module RawAst {
 
     predicate IsType(typ: TypeName) {
       typ in BuiltInTypes || typ in types
+    }
+  }
+
+  // Domains
+
+  datatype Domain = Domain(name: string, params: seq<string>, members: Program)
+  {
+    predicate WellFormed(b3: Program) {
+      members.WellFormed()
     }
   }
 
